SymDiff/Test/resilience/approx_feb_2015/examples/carbin-12/swish/mergedProgSingle.bpl
@@ -178,6 +178,10 @@ function {:inline true} MS$_v1.swish$_v2.swish(_v1.max_r: int,
   _v2.RelaxedEq(_v1.num_r, _v2.num_r)
 }
 
+const {:existential true} __my_houdini_0: bool;
+
+const {:existential true} __my_houdini_1: bool;
+
 function {:inline true} MS_pre_$_v1.swish_loop_anon3_LoopHead$_v2.swish_loop_anon3_LoopHead(_v1.in_N: int, 
     _v1.in_num_r: int, 
     _v1.in_max_r: int, 
@@ -188,7 +192,7 @@ function {:inline true} MS_pre_$_v1.swish_loop_anon3_LoopHead$_v2.swish_loop_ano
     _v2.OK_old: bool)
    : bool
 {
-  _v2.RelaxedEq(_v1.in_max_r, _v2.in_max_r)
+  __my_houdini_0 ==> _v2.RelaxedEq(_v1.in_max_r, _v2.in_max_r)
 }
 
 function {:inline true} MS$_v1.swish_loop_anon3_LoopHead$_v2.swish_loop_anon3_LoopHead(_v1.in_N: int, 
@@ -203,7 +207,7 @@ function {:inline true} MS$_v1.swish_loop_anon3_LoopHead$_v2.swish_loop_anon3_Lo
     _v2.out_num_r: int)
    : bool
 {
-  _v2.RelaxedEq(_v1.out_num_r, _v2.out_num_r)
+  __my_houdini_1 ==> _v2.RelaxedEq(_v1.out_num_r, _v2.out_num_r)
 }
 
 function {:inline true} MS_pre_$_v1.swish$_v2.swish(_v1.max_r: int, 
