SymDiff/Test/resilience/approx_feb_2015/run_symdiff_all_abshoudini.bat
@@ -1,0 +1,34 @@
+@echo off
+
+set INFERENCE=PredicateAbsFull
+REM set INFERENCE=PredicateAbs
+
+pushd examples
+
+echo ---------- control\arr1-absHoudini -----------
+pushd .
+cd control\arr1-absHoudini
+CALL run_symdiff_bpl.cmd v1 v2 /rvt /opts:" -usemutual -asserts -freeContracts -useAbstractHoudiniInference " /inferContracts:"/inlineDepth:1 /abstractHoudini:%INFERENCE% "
+popd
+echo ---------- control\selSort-absHoudini -----------
+pushd .
+cd control\selSort-absHoudini
+CALL run_symdiff_bpl.cmd v1 v2 /rvt /opts:" -usemutual -asserts -freeContracts -useAbstractHoudiniInference " /inferContracts:"/inlineDepth:1 /abstractHoudini:%INFERENCE% "
+popd
+echo ---------- carbin-12\water-absHoudini -----------
+pushd .
+cd carbin-12\water-absHoudini
+CALL run_symdiff_bpl.cmd v1 v2 /rvt /opts:" -usemutual -asserts -freeContracts -useAbstractHoudiniInference " /inferContracts:"/inlineDepth:1 /abstractHoudini:%INFERENCE% "
+popd
+echo ---------- carbin-12\lu-absHoudini -----------
+pushd .
+cd carbin-12\lu-absHoudini
+CALL run_symdiff_bpl.cmd v1 v2 /rvt /opts:" -usemutual -asserts -freeContracts -useAbstractHoudiniInference " /inferContracts:"/inlineDepth:1 /abstractHoudini:%INFERENCE% "
+popd
+echo ---------- carbin-12\swish-absHoudini -----------
+pushd .
+cd carbin-12\swish-absHoudini
+CALL run_symdiff_bpl.cmd v1 v2 /rvt /opts:" -usemutual -asserts -freeContracts -useAbstractHoudiniInference " /inferContracts:"/inlineDepth:1 /abstractHoudini:%INFERENCE% "
+popd
+echo ------
+popd
